this seems annoying

Pdl/Vocab.lean
@@ -12,26 +12,25 @@ structure Vocab where
   progs : Finset Nat
 deriving DecidableEq
 
+-- no simp here!
+instance instMembershipNatVocab : Membership ℕ Vocab := ⟨fun n v => n ∈ v.1 ∨ n ∈ v.2⟩
+
 @[simp]
 def Vocab.union (a : Vocab) (b : Vocab) : Vocab := ⟨a.1 ∪ b.1, a.2 ∪ b.2⟩
 
-instance : Std.Commutative Vocab.union := sorry
+instance : Std.Commutative Vocab.union := by constructor; aesop
 
-instance : Std.Associative Vocab.union := sorry
+instance : Std.Associative Vocab.union := by constructor; aesop
 
-instance : Union Vocab := ⟨Vocab.union⟩
+instance instUnionVocab : Union Vocab := ⟨Vocab.union⟩
 
 @[simp]
 instance : EmptyCollection Vocab := ⟨ ⟨{}, {}⟩ ⟩
 
-@[simp]
-instance : Membership ℕ Vocab := ⟨fun n v => n ∈ v.1 ∨ n ∈ v.2⟩
+class HasVocabulary (α : Type) where
+  voc : α → Vocab
 
-@[simp]
-def Vocab.fromList (l : List Vocab) : Vocab := l.foldr (.union) {}
-
-@[simp]
-def Vocab.fromFinset (X : Finset Vocab) : Vocab := X.fold (Vocab.union) {} id
+open HasVocabulary
 
 mutual
   def vocabOfProgram : Program → Vocab
@@ -48,37 +47,59 @@ mutual
     | ⌈α⌉ φ => vocabOfProgram α ∪ vocabOfFormula φ
 end
 
-@[simp]
-theorem Vocab.props_dist {X Y : Vocab} : (X ∪ Y).props = X.props ∪ Y.props := by sorry
-
-@[simp]
-theorem Vocab.progs_dist {X Y : Vocab} : (X ∪ Y).progs = X.progs ∪ Y.progs := by sorry
-
-def vocabOfSetFormula : Finset Formula → Vocab
-  | X => .fromFinset (X.biUnion (fun f => {vocabOfFormula f}))
-
-def vocabOfListFormula : List Formula → Vocab
-  | X => .fromList (X.map vocabOfFormula)
-
-def vocabOfListProgram : List Program → Vocab
-  | X => .fromList (X.map vocabOfProgram)
-
-@[simp]
-theorem inVocList : n ∈ vocabOfListFormula L ↔ ∃φ ∈ L, n ∈ vocabOfFormula φ := by
-  induction L
-  · simp [vocabOfListFormula]
-  case cons φ L IH =>
-    cases em (n ∈ vocabOfFormula φ) <;> simp_all [vocabOfListFormula]
-    sorry
-
-class HasVocabulary (α : Type) where
-  voc : α → Vocab
-
 instance formulaHasVocabulary : HasVocabulary Formula := ⟨vocabOfFormula⟩
+
 instance programHasVocabulary : HasVocabulary Program := ⟨vocabOfProgram⟩
-instance finsetFormulaHasVocabulary : HasVocabulary (Finset Formula) := ⟨vocabOfSetFormula⟩
-instance listFormulaHasVocabulary : HasVocabulary (List Formula) := ⟨vocabOfListFormula⟩
-instance listProgramHasVocabulary : HasVocabulary (List Program) := ⟨vocabOfListProgram⟩
+
+@[simp]
+theorem Vocab.props_dist {X Y : Vocab} : (X ∪ Y).props = X.props ∪ Y.props := by
+  ext a; simp [instUnionVocab]
+
+@[simp]
+theorem Vocab.progs_dist {X Y : Vocab} : (X ∪ Y).progs = X.progs ∪ Y.progs := by
+  ext a; simp [instUnionVocab]
+
+instance [HasVocabulary α] : HasVocabulary (List α) :=
+  ⟨fun X => (X.map voc).foldr (.union) {}⟩
+
+instance [HasVocabulary α] : HasVocabulary (Finset α) :=
+  ⟨fun X => (X.biUnion (fun f => {voc f})).fold (Vocab.union) {} id ⟩
+
+@[simp]
+theorem inVocList [HasVocabulary α] {L : List α} : n ∈ voc L ↔ ∃ φ ∈ L, n ∈ voc φ := by
+  induction L
+  · simp [voc, instMembershipNatVocab]
+  case cons φ L IH =>
+    cases em (n ∈ voc φ) <;> simp_all [voc, instMembershipNatVocab ]
+    aesop
+
+@[simp]
+theorem voc_mem_union [HasVocabulary α] n (x y : α) :
+      n ∈ voc x ∪ voc y
+    ↔ (n ∈ voc x ∨ n ∈ voc y) := by
+  simp_all [voc, instMembershipNatVocab]
+  tauto
+
+@[simp]
+theorem voc_not_mem_union [HasVocabulary α] {x y : α} :
+      n ∉ voc x ∪ voc y
+    ↔ (n ∉ voc x ∧ n ∉ voc y) := by
+  simp_all [voc, instMembershipNatVocab]
+
+
+@[simp]
+theorem vocabOfFormula_mem_union n (x y : Formula) :
+      n ∈ vocabOfFormula x ∪ vocabOfFormula y
+    ↔ (n ∈ vocabOfFormula x ∨ n ∈ vocabOfFormula y) := by
+  simp_all [instMembershipNatVocab]
+  tauto
+
+@[simp]
+theorem vocabOfProgram_mem_union n (x y : Program) :
+      n ∈ vocabOfProgram x ∪ vocabOfProgram y
+    ↔ (n ∈ vocabOfProgram x ∨ n ∈ vocabOfProgram y) := by
+  simp_all [instMembershipNatVocab]
+  tauto
 
 /-- Test(α) -/
 def testsOfProgram : Program → List Formula
