Pdl/Fresh.lean
@@ -23,34 +23,40 @@ open HasVocabulary
 mutual
 theorem freshVarForm_is_larger (φ) : ∀ n ∈ voc φ, n < freshVarForm φ := by
   cases φ
-  all_goals simp [freshVarForm, voc, vocabOfFormula, not_or]
+  all_goals simp [freshVarForm, voc, vocabOfFormula, not_or, instMembershipNatVocab]
   case neg φ =>
     apply freshVarForm_is_larger
   case and φ1 φ2 =>
     have IH1 := freshVarForm_is_larger φ1
     have IH2 := freshVarForm_is_larger φ2
+    simp_all [instMembershipNatVocab]
     aesop
   case box α φ =>
     have IHφ := freshVarForm_is_larger φ
     have IHα := freshVarProg_is_larger α
+    simp_all [instMembershipNatVocab]
     aesop
 
 theorem freshVarProg_is_larger (α) : ∀ n ∈ voc α, n < freshVarProg α := by
   cases α
-  all_goals simp [freshVarProg, voc, vocabOfProgram]
+  all_goals simp [freshVarProg, voc, vocabOfProgram, instMembershipNatVocab]
   case union α β =>
     have IHα := freshVarProg_is_larger α
     have IHβ := freshVarProg_is_larger β
+    simp_all [instMembershipNatVocab]
     aesop
   case sequence α β =>
     have IHα := freshVarProg_is_larger α
     have IHβ := freshVarProg_is_larger β
+    simp_all [instMembershipNatVocab]
     aesop
   case star α =>
     have IHα := freshVarProg_is_larger α
+    simp_all [instMembershipNatVocab]
     aesop
   case test φ =>
     have IHφ := freshVarForm_is_larger φ
+    simp_all [instMembershipNatVocab]
     aesop
 end
 
